theories/elpi_prop.v
@@ -4,8 +4,6 @@ From elpi.apps Require Import derive derive.std.
 From HB Require Import structures.
 From det Require Import zify_ssreflect.
 
-Import Language.
-
 Section NurProp.
   Variable u: Unif.
 
