theories/elpi_valid_state.v
@@ -4,7 +4,6 @@ From elpi.apps Require Import derive derive.std.
 From HB Require Import structures.
 From det Require Import zify_ssreflect.
 
-Import Language.
 
 Section NurValidState.
   Variable u : Unif.
