theories/lang.v
@@ -6,88 +6,79 @@ Notation "[subst]" := ltac:(subst).
 Notation "[subst1]" := ltac:(move=> ?;subst).
 Notation "[subst2]" := ltac:(move=> ??;subst).
 
-Module Language.
-  Inductive D := Func | Pred.
-  Inductive B := Exp | d of D.
-  Inductive mode := i |o.
-  Inductive S :=  b of B | arr of mode & S & S.
-  Notation "x '--i-->' y" := (arr i x y) (at level 3).
-  Notation "x '--o-->' y" := (arr o x y) (at level 3).
+Inductive D := Func | Pred.
+Inductive B := Exp | d of D.
+Inductive mode := i |o.
+Inductive S :=  b of B | arr of mode & S & S.
+Notation "x '--i-->' y" := (arr i x y) (at level 3).
+Notation "x '--o-->' y" := (arr o x y) (at level 3).
 
-  Definition P := nat.
-  derive P.
-  Elpi derive.eqbOK.register_axiom P is_P is_nat_inhab P_eqb P_eqb_correct P_eqb_refl.
+Definition P := nat.
+derive P.
+Elpi derive.eqbOK.register_axiom P is_P is_nat_inhab P_eqb P_eqb_correct P_eqb_refl.
 
-  Definition K := nat.
-  derive K.
-  Elpi derive.eqbOK.register_axiom K is_K is_nat_inhab K_eqb K_eqb_correct K_eqb_refl.
+Definition K := nat.
+derive K.
+Elpi derive.eqbOK.register_axiom K is_K is_nat_inhab K_eqb K_eqb_correct K_eqb_refl.
 
-  Definition V := nat.
-  derive V.
-  Elpi derive.eqbOK.register_axiom V is_V is_nat_inhab V_eqb V_eqb_correct V_eqb_refl.
+Definition V := nat.
+derive V.
+Elpi derive.eqbOK.register_axiom V is_V is_nat_inhab V_eqb V_eqb_correct V_eqb_refl.
 
-  Inductive C := 
-    | p of P 
-    | v of V
-    .
-  derive C.
+Inductive C := 
+  | p of P 
+  | v of V
+  .
+derive C.
 
-  Inductive Tm := 
-    | Code : C -> Tm
-    | Data : K -> Tm
-    | Comb : Tm -> Tm -> Tm.
-    (* | Lam  : V -> S -> Tm -> S -> Tm. *)
-  derive Tm.
+Inductive Tm := 
+  | Code : C -> Tm
+  | Data : K -> Tm
+  | Comb : Tm -> Tm -> Tm.
+  (* | Lam  : V -> S -> Tm -> S -> Tm. *)
+derive Tm.
 
-  Record R_ {A} := mkR { head : Tm; premises : list A }.
-  Arguments mkR {_} _ _.
-  derive R_.
-  Inductive A :=
-    | Cut
-    | Call : Tm -> A.
-  derive A.
+Record R_ {A} := mkR { head : Tm; premises : list A }.
+Arguments mkR {_} _ _.
+derive R_.
+Inductive A :=
+  | Cut
+  | Call : Tm -> A.
+derive A.
 
-    (* | PiImpl : V -> R_ A -> A -> A. *)
-  Notation R := (@R_ A).
+  (* | PiImpl : V -> R_ A -> A -> A. *)
+Notation R := (@R_ A).
 
-  HB.instance Definition _ := hasDecEq.Build Tm Tm_eqb_OK.
-  HB.instance Definition _ := hasDecEq.Build A A_eqb_OK.
-  HB.instance Definition _ := hasDecEq.Build C C_eqb_OK.
-  HB.instance Definition _ := hasDecEq.Build P P_eqb_OK.
-  HB.instance Definition _ := hasDecEq.Build K K_eqb_OK.
-  HB.instance Definition _ := hasDecEq.Build V V_eqb_OK.
-  HB.instance Definition _ := hasDecEq.Build R (R__eqb_OK _ _ A_eqb_OK).
+HB.instance Definition _ := hasDecEq.Build Tm Tm_eqb_OK.
+HB.instance Definition _ := hasDecEq.Build A A_eqb_OK.
+HB.instance Definition _ := hasDecEq.Build C C_eqb_OK.
+HB.instance Definition _ := hasDecEq.Build P P_eqb_OK.
+HB.instance Definition _ := hasDecEq.Build K K_eqb_OK.
+HB.instance Definition _ := hasDecEq.Build V V_eqb_OK.
+HB.instance Definition _ := hasDecEq.Build R (R__eqb_OK _ _ A_eqb_OK).
 
-  Record Sigma := { sigma : V -> option Tm }.
-  Definition empty : Sigma := {| sigma := fun _ => None |}.
+Record Sigma := { sigma : V -> option Tm }.
+Definition empty : Sigma := {| sigma := fun _ => None |}.
 
-  Definition index := list R.
-  Definition mode_ctx := Tm -> list mode.
-  Definition sigT := P -> S.
-  (* 
-    The predicate knows about the signature of all predicates, therefore,
-    for each predicate we return a S (not an option S)
-  *)
-  Record program := { (*depth : nat;*) rules : index; modes : mode_ctx; sig : sigT }.
+Definition index := list R.
+Definition mode_ctx := Tm -> list mode.
+Definition sigT := P -> S.
+(* 
+  The predicate knows about the signature of all predicates, therefore,
+  for each predicate we return a S (not an option S)
+*)
+Record program := { (*depth : nat;*) rules : index; modes : mode_ctx; sig : sigT }.
 
-  Parameter program_eqb : program -> program -> bool.
-  Parameter is_program : program -> Type.
-  Parameter is_program_inhab : forall p : program, is_program p.
-  Parameter program_eqb_correct : forall p1 p2, program_eqb p1 p2 -> p1 = p2.
-  Parameter program_eqb_refl : forall x, program_eqb x x.
+Parameter program_eqb : program -> program -> bool.
+Parameter is_program : program -> Type.
+Parameter is_program_inhab : forall p : program, is_program p.
+Parameter program_eqb_correct : forall p1 p2, program_eqb p1 p2 -> p1 = p2.
+Parameter program_eqb_refl : forall x, program_eqb x x.
 
-  Parameter Sigma_eqb : Sigma -> Sigma -> bool.
-  Parameter is_Sigma : Sigma -> Type.
-  Parameter is_Sigma_inhab : forall p : Sigma, is_Sigma p.
-  Parameter Sigma_eqb_correct : forall p1 p2, Sigma_eqb p1 p2 -> p1 = p2.
-  Parameter Sigma_eqb_refl : forall x, Sigma_eqb x x.
-
-End Language.
-
-Module Type Unif.
-  Import Language.
-  Parameter unify : Tm -> Tm -> Sigma -> option Sigma.
-  Parameter matching : Tm -> Tm -> Sigma -> option Sigma.
-End Unif.
+Parameter Sigma_eqb : Sigma -> Sigma -> bool.
+Parameter is_Sigma : Sigma -> Type.
+Parameter is_Sigma_inhab : forall p : Sigma, is_Sigma p.
+Parameter Sigma_eqb_correct : forall p1 p2, Sigma_eqb p1 p2 -> p1 = p2.
+Parameter Sigma_eqb_refl : forall x, Sigma_eqb x x.
 
 
