theories/test.v
@@ -1,0 +1,14 @@
+From mathcomp Require Import all_ssreflect.
+From det Require Import lang run run_prop valid_state elpi elpi_prop elpi_valid_state elpi_equiv.
+From elpi.apps Require Import derive derive.std.
+From HB Require Import structures.
+From det Require Import zify_ssreflect.
+
+Section main.
+  Variable u: Unif.
+
+  Lemma xx x xs s' r:
+    valid_ca (x:::xs) -> nur u x.1 x.2 xs s' r -> valid_ca r.
+  Proof.
+    move=> H1 H2.
+    apply: valid_state_valid_ca.                           
